theories/check.v
@@ -57,526 +57,174 @@ Proof.
   - move=> s []//= _ ???? _ _ [_ ->] <-/=; repeat eexists; rewrite ?minD_refl//.
     (* apply: sV_expand_refl. *)
   - move=> s INIT A sB B HINIT dA IH sV sV' r d ign H/=.
-    rewrite is_dead_next_alt//= => dtB<-{r}.
+    case dtA: (tc_tree_aux _ _ A) => /=[[DA' sVA]|]//=.
+    case dtB: (tc_tree_aux _ _ B) => /=[[DB sVB]|]//=.
+    case M: merge_sig => //=[m][??]<-{r}; subst.
+    rewrite //=get_tree_Or/= is_dead_has_cut//=.
     have ?: sB = s by admit.
     subst.
-    have:= IH _ _ _ _ _ _ _ erefl.
-    move=> /(_ _ _ _ _ H dtB).
-    move=> [S[d' [H1 H2]]].
-    rewrite get_tree_Or/= is_dead_next_alt//= H2.
-    by repeat eexists; eauto.
+    have {IH}[S[d' [H1 H2]]]:= IH _ _ _ _ _ H dtB erefl.
+    have:= same_ty_tc_tree_aux sP sV A ign Pred.
+    rewrite dtA/=.
+    case dtA': tc_tree_aux => //=[[D S']]/eqP[?]; subst.
+    remember ((get_tree _)) as T eqn:HT.
+    have:= same_ty_tc_tree_aux sP sV T DB Pred.
+    rewrite H2/=.
+    case dtB': tc_tree_aux => //=[[D1 S1]]/eqP[?]; subst.
+    admit.
   - move=> s INIT A sB B HINIT dA IH A' eA sV sV' r d ign H/=.
     have fA:= expand_not_failed _ eA notF.
-    rewrite next_alt_not_failed//=.
     move=> + <-{r}/=.
-    case nB: next_alt => [B'|]//=.
-      case dtA: (tc_tree_aux _ _ A) => /=[[DA' sVA]|]//=.
-      case dtB: (tc_tree_aux _ _ B) => /=[[DB sVB]|]//=.
-      case M: merge_sig => //=[S']; subst.
-      have {IH}/=[S[d'[H1 H2]]]:= IH _ _ _ _ _ H dtA eA.
-      move=> [??]; subst.
-      case nA: next_alt => [A''|]//=; last first.
-        have:= same_ty_tc_tree_aux sP sV B ign (if has_cut A then maxD DA' DB else Pred).
-        rewrite dtB/=; case dtB': tc_tree_aux => //=[[D' sVx]] /eqP[?]; subst sVx.
-        repeat eexists.
-        move: dtB'.
-        case: ifP => //=cA.
-        case N: maxD => //=.
-        destruct DA', DB => //=.
-        have [[] [//= _ {}H]] := tc_tree_aux_func2 dtB.
-        rewrite H; congruence.
-      have:= same_ty_tc_tree_aux sP sV A' DA'(if has_cut A then maxD DA' DB else Pred).
-      rewrite H2; case dtA' : tc_tree_aux => //=[[Dx Sx]] /eqP[?]; subst Sx.
-      have:= same_ty_tc_tree_aux sP sV B ign (if has_cut A then maxD DA' DB else Pred).
-      rewrite dtB/=; case dtB': tc_tree_aux => //=[[Dy Sy]] /eqP[?]; subst Sy.
-      case M1: merge_sig => /=[S'|].
-        repeat eexists.
-        move: dtB' dtA'.
-        case: ifP => cA//.
-        destruct DA' => //=.
-        destruct DB => //=.
-        rewrite H2 => +[?]; subst.
-        have [[][//_ Hz]] := tc_tree_aux_func2 dtB.
-        rewrite Hz => -[?]; subst; rewrite maxD_comm/=.
-        simpl in H1; subst.
-        rewrite (expand_Exp_has_cut _ eA)//=.
-      (* BELOW: SHOULD NOT BE REACHABLE: merge_sig S sVB is a ty_ok *)
-      (* sV1 <= sVA
-          sV1 <= sVB
-          sVA + sVB = sV2
-          sV1 <= S 
-          ==========> 
-          goal: merge_sig S sVB = ty_ok
-          IDEA: all vars in S have "compatible" with sVA
-          and all variables not appearing in sVA are also not in sVB, i.e. they are fresh
-
-          FORMALLY:
-          forall x \in S, if x \in sVA, then they are compatible,
-                          else x is not in sVB
-      *)
-      idtac.
-      admit.
-    move=> H2.
-    have /=[S[d' [H3 H4]]]  := IH _ _ _ _ _ H H2 eA.
-    rewrite H4/=.
-    have /= [d1[MM ->]]:= next_alt_None_dt sP sV d nB.
-    case: eqP => Hz; repeat eexists; auto.
+    (* case nB: next_alt => [B'|]//=. *)
+    case dtA: (tc_tree_aux _ _ A) => /=[[DA' sVA]|]//=.
+    case dtB: (tc_tree_aux _ _ B) => /=[[DB sVB]|]//=.
+    case M: merge_sig => //=[S']; subst.
+    have {IH}/=[S[d'[H1 H2]]]:= IH _ _ _ _ _ H dtA eA.
+    move=> [??]; subst.
+    rewrite (expand_Exp_has_cut eA).
+    admit.
   - move=> s INIT A sB B HINIT dA IH A' eA sV sV' r d ign H/=.
     have fA:= expand_not_failed _ eA notF.
-    rewrite next_alt_not_failed//=.
-    move=> + <-{r}/=.
-    rewrite (is_ko_tc_tree_aux is_ko_cutr)/=(is_ko_next_alt _ is_ko_cutr)/=.
-    case nB: next_alt => [B'|]//=.
-      case dtA: (tc_tree_aux _ _ A) => /=[[DA' sVA]|]//=.
-      case dtB: (tc_tree_aux _ _ B) => /=[[DB sVB]|]//=.
-      case M: merge_sig => //=[S']; subst.
-      move=> [??]; subst.
-      have /=[S[d' [H1 H2]]] := IH _ _ _ _ _ H dtA eA.
-      have := same_ty_tc_tree_aux sP sV A' DA' (if has_cut A then maxD DA' DB else Pred).
-      rewrite H2/= => /eqP.
-      case Hz : tc_tree_aux => //=[[Dx sX]][?]; subst sX.
-      case: eqP; repeat eexists; rewrite //=?minD_refl//=.
-      move: Hz.
-      case:ifP => //= cA.
-      destruct DA'; simpl in *; subst => //.
-      destruct DB => //=; congruence.
-    move=> H2.
-    have /=[S[d' [H0 H1]]]  := IH _ _ _ _ _ H H2 eA.
-    rewrite H1/=.
-    by case:ifP => //=; repeat eexists; auto; rewrite minD_refl.
+    case dtA: (tc_tree_aux _ _ A) => /=[[DA' sVA]|]//=.
+    case dtB: (tc_tree_aux _ _ B) => /=[[DB sVB]|]//=.
+    case M: merge_sig => //=[S']; subst.
+    move=> [??]; subst.
+    have {IH}/=[S[d' [H1 H2]]] := IH _ _ _ _ _ H dtA eA.
+    have := same_ty_tc_tree_aux sP sV A' DA' (if has_cut A then maxD DA' DB else Pred).
+    rewrite H2/= => /eqP.
+    case Hz : tc_tree_aux => //=[[Dx sX]][?]; subst sX.
+    move=> <-{r}/=.
+    rewrite Hz/=.
+    admit.
   - move=> s INIT A sB B HINIT dA IH A' eA sV sV' r d ign H/=.
     have [? fA] := expand_failed_same _ eA; subst A'.
     move=> +<-{r}/=.
-    case nA: next_alt => [A'|]//=; last first.
-      move=> H2.
-      have := same_ty_tc_tree_aux sP sV B ign d.
-      rewrite H2/=; case H3: tc_tree_aux => /=[[D1 Sx]|] => //=/eqP[?]; subst Sx.
-      repeat eexists.
-      destruct d => //=.
-      have [d2[H4 H5]]:= tc_tree_aux_func2 H2.
-      destruct d2 => //=.
-      congruence.
-    case nB: next_alt => [B'|]//=; last first.
-      move=> H2.
-      have [d2[H3 H4]]:= tc_tree_aux_func2 H2.
-      rewrite minD_comm in H3.
-      destruct d; simpl in H3; subst.
-        by rewrite H4; repeat eexists.
-      move=>/=.
-      have := same_ty_tc_tree_aux sP sV A ign Pred.
-      by rewrite H2/=; case: tc_tree_aux => //= -[]//=; repeat eexists.
-    case dtA: (tc_tree_aux _ _ A) => /=[[DA' sVA]|]//=.
-    case dtB: (tc_tree_aux _ _ B) => /=[[DB sVB]|]//=.
+    have:= same_ty_tc_tree_aux sP sV A ign d.
+    case dtA1: (tc_tree_aux _ _ A) => /=[[DA1 sVA1]|]//=.
+    case dtA2: (tc_tree_aux _ _ A) => /=[[DA2 sVA2]|]//=/eqP[?]; subst sVA2.
+    have:= same_ty_tc_tree_aux sP sV B ign d.
+    case dtB1: (tc_tree_aux _ _ B) => /=[[DB1 sVB1]|]//=.
+    case dtB2: (tc_tree_aux _ _ B) => /=[[DB2 sVB2]|]//=/eqP[?]; subst sVB2.
     case M: merge_sig => //=[S'][??]; subst.
-    pose X := if has_cut A then maxD DA' DB else Pred.
-    rewrite -/X.
-    have := same_ty_tc_tree_aux sP sV A ign X.
-    rewrite dtA; case dtA': tc_tree_aux => //=[[d' blah]]/eqP[?]; subst blah.
-    have := same_ty_tc_tree_aux sP sV B ign X.
-    rewrite dtB; case dtB': tc_tree_aux => //=[[d1 blah]]/eqP[?]; subst blah.
-    rewrite M/=; repeat eexists.
-    move: dtA' dtB'; rewrite/X.
-    case:ifP => // c.
-    destruct DA' => //=.
-    destruct DB => //=.
-    have [[][//_ ->]] := tc_tree_aux_func2 dtA.
-    move=> [?]; subst => /=.
-    have [[][//_ ->]] := tc_tree_aux_func2 dtB; congruence.
+    repeat eexists; case:ifP => //=.
+    rewrite failed_has_cut//=.
   - move=> s INIT A sB B HINIT dA IH A' eA sV sV' r d ign H/=.
     have [? sA]:= expand_solved_same _ eA; subst A'.
     move=> +<-{r}/=.
-    rewrite next_alt_not_failed?success_failed//=.
-    case nB: next_alt => [B'|]//=; last first.
-      move=> H2; have [d2[H3 H4]] := tc_tree_aux_func2 H2.
-      have := same_ty_tc_tree_aux sP sV A ign d.
-      rewrite H2; case dtA': tc_tree_aux => //=[[d' blah]]/eqP[?]; subst blah.
-      repeat eexists; destruct d2; simpl in H3; subst => //.
-      destruct d => //=; congruence.
-    case dtA: (tc_tree_aux _ _ A) => /=[[DA' sVA]|]//=.
-    case dtB: (tc_tree_aux _ _ B) => /=[[DB sVB]|]//=.
+    rewrite success_has_cut//=.
+    have:= same_ty_tc_tree_aux sP sV A ign d.
+    case dtA1: (tc_tree_aux _ _ A) => /=[[DA1 sVA1]|]//=.
+    case dtA2: (tc_tree_aux _ _ A) => /=[[DA2 sVA2]|]//=/eqP[?]; subst sVA2.
+    have:= same_ty_tc_tree_aux sP sV B ign d.
+    case dtB1: (tc_tree_aux _ _ B) => /=[[DB1 sVB1]|]//=.
+    case dtB2: (tc_tree_aux _ _ B) => /=[[DB2 sVB2]|]//=/eqP[?]; subst sVB2.
     case M: merge_sig => //=[S'][??]; subst.
-    have [d2[H2 H3]] := tc_tree_aux_func2 dtB.
-    have [d3[H4 H5]]:= tc_tree_aux_func2 dtA.
-    pose X := if has_cut A then maxD DA' DB else Pred.
-    rewrite -/X.
-    have := same_ty_tc_tree_aux sP sV A ign X.
-    rewrite dtA; case dtA': tc_tree_aux => //=[[d' blah]]/eqP[?]; subst blah.
-    have := same_ty_tc_tree_aux sP sV B ign X.
-    rewrite dtB; case dtB': tc_tree_aux => //=[[d1 blah]]/eqP[?]; subst blah.
-    rewrite M/=; repeat eexists.
-    move: dtA' dtB'; rewrite/X.
-    case:ifP => // c.
-    destruct DA' => //=.
-    destruct DB => //=.
-    have [[][//_ ->]] := tc_tree_aux_func2 dtA.
-    move=> [?]; subst => /=.
-    have [[][//_ ->]] := tc_tree_aux_func2 dtB; congruence.
-  - move=> s INIT A B0 B HINIT IH A' eA sV sV' r d ign H/=.
+    repeat eexists.
+  - move=> s INIT A B0 B HINIT IH A' eA sV sV' r d ign H/= + <-/=.
     have fA:= expand_not_failed _ eA notF.
     have sA:= expand_not_solved_not_success _ eA notF.
-    rewrite fA (next_alt_not_failed fA)//= sA/=.
-    move=> + <-{r}/=.
-    case nB0: next_alt => [B0'|]//=.
-      case dtA: (tc_tree_aux _ _ A) => /=[[DA' sVA]|]//=.
-      case dtB0: (tc_tree_aux _ _ B0) => /=[[DB0 sVB0]|]//=.
-      case dtB: (tc_tree_aux _ _ B) => /=[[DB sVB]|]//=.
-      case M: merge_sig => //=[S'][??]; subst.
-      rewrite orbF andbF/=.
-      have {IH}/=[S[d'[H4 H5]]] := IH _ _ _ _ _ H dtA eA.
-      case nA: next_alt => [A''|]//=; last first.
-        repeat eexists; rewrite minD_refl//.
-      have [d0[//H2 H3]] := tc_tree_aux_func2 dtB.
-      case: ifP => fA'.
-        have := same_ty_tc_tree_aux sP sV A' DA' (maxD DB0 DB).
-        rewrite H5; case dtA': tc_tree_aux => //=[[d2 blah]]/eqP[?]; subst blah.
-        (* in S there are more assignemnts than in sV *)
-        (* all of this new assigments will never appear in B0
-            all output are the same more precise
-        *)
-        admit. (*PB WITH SIG*)
-      rewrite orbF.
-      case: ifP.
-        move=> /andP[sA' /eqP nA'].
-        have [dd[//H6 H7]] := next_alt_None_dt sP sV (maxD DB0 DB) nA'.
-        rewrite H7/=.
-        case nB: next_alt => [B'|]//=; last first.
-          by repeat eexists; rewrite minD_refl.
-        (* (DEAD \/ (OK /\ ... ! /\ ... OK) \/ Any) /\ B  -> OK /\ B *)
-        admit. (*PB WITH SIG*)
-      have := same_ty_tc_tree_aux sP sV A' DA' (maxD DB0 DB).
-      rewrite H5; case dtA': tc_tree_aux => //=[[d2 blah]]/eqP[?]; subst blah.
-      case sA' : success => //=.
-        move=> {nA A''}.
-        case nA: next_alt => [A''|]//= _.
-        admit. (*PB WITH SIG*)
-      move=> _.
-      admit. (*PB WITH SIG*)
-    case nB: next_alt => [B'|]//=.
-      case dtA: (tc_tree_aux _ _ A) => /=[[DA' sVA]|]//=.
-      case dtB0: (tc_tree_aux _ _ B0) => /=[[DB0 sVB0]|]//=.
-      case dtB: (tc_tree_aux _ _ B) => /=[[DB sVB]|]//=.
-      case M: merge_sig => //=[S'][??]; subst.
-      rewrite orbF andbT.
-      case nA: next_alt => [A''|]//=; last first; rewrite?orbF?orbT/=.
-        repeat eexists; rewrite minD_refl//.
-      rewrite andbT.
-      case: ifP => fA'.
-        repeat eexists; rewrite minD_refl//.
-      rewrite fA'.
-      have [dd[//H2 H3]] := tc_tree_aux_func2 dtB.
-      have [d2[H4 H5]] := tc_tree_aux_func2 dtA.
-      have {IH}/=[S[d'[H6 H7]]] := IH _ _ _ _ _ H dtA eA.
-      have := same_ty_tc_tree_aux sP sV A' DA' (maxD DB0 DB).
-      rewrite H7; case dtA': tc_tree_aux => //=[[d3 blah]]/eqP[?]; subst blah.
-      case: ifP => sA'.
-        admit. (*PB WITH SIG*)
-      admit. (*PB WITH SIG*)
-    move=> [??]; subst.
-    rewrite andbT orbT; repeat eexists; rewrite minD_refl//.
+    case dtA1: (tc_tree_aux _ _ A) => /=[[DA1 sVA1]|]//=.
+    case dtB01: (tc_tree_aux _ _ B0) => /=[[DB01 sVB01]|]//=.
+    case dtB1: (tc_tree_aux _ _ B) => /=[[DB1 sVB1]|]//=.
+    case M: merge_sig => //=[S'][??]; subst.
+    have {IH}/=[S[d'[H1 H2]]] := IH _ _ _ _ _ H dtA1 eA.
+    admit.
   - move=> s INIT A B0 B HINIT IH A' eA sV sV' r d ign H/=.
-    have fA:= expand_not_failed _ eA notF.
-    have sA:= expand_not_solved_not_success _ eA notF.
-    rewrite fA (next_alt_not_failed fA)//= sA/= => +<-{r}/=.
-    case nB0: next_alt => [B0'|]//=.
-      case dtA: (tc_tree_aux _ _ A) => /=[[DA' sVA]|]//=.
-      case dtB0: (tc_tree_aux _ _ B0) => /=[[DB0 sVB0]|]//=.
-      case dtB: (tc_tree_aux _ _ B) => /=[[DB sVB]|]//=.
-      case M: merge_sig => //=[S'][??]; subst.
-      rewrite orbF andbF/=.
-      case nA: next_alt => [A''|]//=; last first.
-        by repeat eexists; rewrite minD_refl.
-      have [xx[//H2 H3]] := tc_tree_aux_func2 dtB.
-      have /=[S[d'[H4 H5]]] := IH _ _ _ _ _ H dtA eA.
-      have := same_ty_tc_tree_aux sP sV A' DA' (maxD DB0 DB).
-      rewrite H5; case dtA': tc_tree_aux => //=[[d2 blah]]/eqP[?]; subst blah.
-      case: ifP => fA'.
-        admit. (*PB WITH SIG*)
-      rewrite orbF/=.
-      case:ifP => H1/=.
-        case:ifP.
-          repeat eexists; rewrite minD_refl//.
-        move=> /eqP nB.
-        admit. (*PB WITH SIG*)
-      admit. (*PB WITH SIG*)
-    rewrite !orbT/=!andbT/=.
-    case nB: next_alt => [B'|]//=; rewrite?orbF ?orbT/=; last first.
-      by move=> [??]; subst; repeat eexists; rewrite minD_refl.
     case dtA: (tc_tree_aux _ _ A) => /=[[DA' sVA]|]//=.
     case dtB0: (tc_tree_aux _ _ B0) => /=[[DB0 sVB0]|]//=.
     case dtB: (tc_tree_aux _ _ B) => /=[[DB sVB]|]//=.
     case M: merge_sig => //=[S'][??]; subst.
-    case fA': failed => /=.
-      repeat eexists.
-      by rewrite minD_refl.
-    rewrite next_alt_not_failed//=.
-    case:ifP => sA'.
-      admit. (*PB WITH SIG*)
-    have /=[S[d'[H4 H5]]] := IH _ _ _ _ _ H dtA eA.
-    have := same_ty_tc_tree_aux sP sV A' DA' (maxD DB0 DB).
-    rewrite H5; case dtA': tc_tree_aux => //=[[d2 blah]]/eqP[?]; subst blah.
-    admit. (*PB WITH SIG*)
+    move=> <-{r}/=.
+    admit.
   - move=> s INIT A B0 B HINIT IH A' eA sV sV' r d ign H/=.
     have [? fA]:= expand_failed_same _ eA; subst A' => +<-{r}/=.
-    rewrite fA/=.
-    case:ifP => H1.
-      move=> [??]; subst.
-      by repeat eexists; rewrite minD_refl.
-    case dtA: (tc_tree_aux _ _ A) => /=[[DA' sVA]|]//= dtB0.
-    have:= same_ty_tc_tree_aux sP sV A ign d.
-    rewrite dtA; case dtA' : tc_tree_aux => /=[[DA'' blah]|]//=/eqP[?]; subst blah.
-    have:= same_ty_tc_tree_aux sP sVA B0 DA' DA''.
-    rewrite dtB0; case dtB0' : tc_tree_aux => /=[[DB0'' blah]|]//=/eqP[?]; subst blah.
-    repeat eexists.
-    destruct d => //=.
-    move: H1.
-    case nB0: next_alt => [B0'|]//=; rewrite orbF.
-    case nA: next_alt => [A'|]//= _.
-    have /=[S[d'[H4 H5]]] := IH _ _ _ _ _ H dtA eA.
-    destruct DA'; destruct DA''; simpl in H4; try congruence.
-    have [[][//_]] := tc_tree_aux_func2 dtB0; congruence.
-  - move=> s INIT A B0 B HINIT HL A' eA HR sV sV' r d ign H/=.
-    have [? sA]:= expand_solved_same _ eA; subst A'.
-    have fA:= success_failed _ sA.
-    rewrite sA fA (next_alt_not_failed fA)/=.
-    case e1: step => //=[B'|B'|B'|B'].
-    - have fB:= expand_not_failed _ e1 notF.
-      have sB:= expand_not_solved_not_success _ e1 notF.
-      rewrite (next_alt_not_failed fB)//= andbF/=.
-      move=> + <-{r}/=; rewrite fA sA/= (next_alt_not_failed fA)/=.
-      case nA: next_alt => [A'|]//=.
-        case nB0: next_alt => [B0'|]//=.
-          case dtA: (tc_tree_aux _ _ A) => /=[[DA' sVA]|]//=.
-          case dtB0: (tc_tree_aux _ _ B0) => /=[[DB0 sVB0]|]//=.
-          case dtB: (tc_tree_aux _ _ B) => /=[[DB sVB]|]//=.
-          case M: merge_sig => //=[S'][??]; subst.
-          have := same_ty_tc_tree_aux sP sV A ign (maxD DB0 DB).
-          rewrite dtA; case dtA': tc_tree_aux => //=[[d2 blah]]/eqP[?]; subst blah.
-          
-          have := same_ty_tc_tree_aux sP sVA B0 DA' d2.
-          rewrite dtB0; case dtB0': tc_tree_aux => //=[[d3 blah]]/eqP[?]; subst blah.
-
-          have /= := HR _ _ _ _ _ _ dtB e1.
-          (*PB WITH IH*)
-          admit.
-        move=> dtB.
-        case nB: next_alt => [B''|]//=.
-          apply: HR _ _ _ _ _ _ dtB e1.
-          admit. (*PB WITH IH*)
-        repeat eexists; rewrite minD_refl//.
-      case nB0: next_alt => [B0'|]//=.
-        case dtA: (tc_tree_aux _ _ A) => /=[[DA' sVA]|]//=dtB.
-        have := same_ty_tc_tree_aux sP sV A ign d.
-        rewrite dtA; case dtA': tc_tree_aux => //=[[d2 blah]]/eqP[?]; subst blah.
-        case:eqP => nB'.
-          by repeat eexists; rewrite minD_refl.
-        admit.
-      move=> dtB.
-      case nB: next_alt => [B''|]//=.
-        apply: HR dtB e1.
-        admit.
-      repeat eexists; rewrite minD_refl//.
-    - have fB:= expand_not_failed _ e1 notF.
-      have sB:= expand_not_solved_not_success _ e1 notF.
-      rewrite (next_alt_not_failed fB)//= andbF/=.
-      move=> + <-{r}/=.
-      rewrite (is_ko_next_alt _ is_ko_cutr)/=.
-      rewrite failed_success_cut success_cut sA/=next_alt_cutl/=.
-      rewrite (@next_alt_not_failed (cutl A))/=; last first.
-        rewrite failed_success_cut success_cut sA//.
-      case nA: next_alt => [A'|]//=.
-        case nB0: next_alt => [B0'|]//=.
-          case dtA: (tc_tree_aux _ _ A) => /=[[DA' sVA]|]//=.
-          case dtB0: (tc_tree_aux _ _ B0) => /=[[DB0 sVB0]|]//=.
-          case dtB: (tc_tree_aux _ _ B) => /=[[DB sVB]|]//=.
-          case M: merge_sig => //=[S'][??]; subst.
-          case: eqP => nB'.
-            by repeat eexists; rewrite minD_refl//.
-          admit.
-        move=> H1.
-        case nB: next_alt => [B''|]/=; last first.
-          by repeat eexists; rewrite minD_refl.
-        apply: HR _ _ _ _ _ _ H1 e1.
-        admit.
-      case nB0: next_alt => [B0'|]//=.
-        case dtA: (tc_tree_aux _ _ A) => /=[[DA' sVA]|]//=.
-        case dtB: (tc_tree_aux _ _ B) => /=[[DB sVB]|]//=[??]; subst.
-        case nB: next_alt => [B''|]/=; last first.
-          by repeat eexists; rewrite minD_refl.
-        have [d1[H1]] := next_alt_None_dt sP sV ign nA.
-        rewrite dtA => -[??]; subst.
-        apply: HR dtB e1.
-        admit.
-      move=> dtB.
-      case nB: next_alt => [B''|]/=; last first.
-        by repeat eexists; rewrite minD_refl.
-      apply: HR dtB e1.
+    case dtA: (tc_tree_aux _ _ A) => /=[[DA' sVA]|]//=.
+    case dtB0: (tc_tree_aux _ _ B0) => /=[[DB0 sVB0]|]//=.
+    case dtB: (tc_tree_aux _ _ B) => /=[[DB sVB]|]//=.
+    case M: merge_sig => //=[S'][??]; subst.
+    have:= same_ty_tc_tree_aux sP sV A ign (maxD DB0 DB).
+    rewrite dtA.
+    case dtA1: (tc_tree_aux _ _ A) => /=[[DA1 sVA1]|]//=/eqP[?]; subst sVA1.
+    have:= same_ty_tc_tree_aux sP sVA B DA' DA1.
+    rewrite dtB/=.
+    case dtB1: (tc_tree_aux _ _ B) => /=[[DB1 sVB1]|]//=/eqP[?]; subst sVB1.
+    have:= same_ty_tc_tree_aux sP sVA B0 DA' DA1.
+    rewrite dtB0/=.
+    case dtB01: (tc_tree_aux _ _ B0) => /=[[DB01 sVB01]|]//=/eqP[?]; subst sVB01.
+    rewrite M/=; repeat eexists.
+    destruct DB0,DB => //=; simpl in *.
+    destruct DA'; simpl in *; last first.
+      have [[][// _ H1]] := tc_tree_aux_func2 dtB0.
+      move: dtB01; destruct DA1; rewrite ?dtB0?H1 => -[<-]/=; [|congruence].
+      have [[][// _ H2]] := tc_tree_aux_func2 dtB; congruence.
+    destruct ign.
+      move: dtA1; rewrite dtA => -[?]; subst.
+      move: dtB01; rewrite dtB0 => -[<-]/=; congruence.
+    have [[][//= _]] := tc_tree_aux_func2 dtA.
+    rewrite dtA1 => -[?]; subst.
+    destruct DB01;[|congruence] => /=; congruence.
+  - move=> s INIT A B0 B HINIT HL A' eA HR sV sV' r d ign H/= + <-{r}/=.
+    case dtA: (tc_tree_aux _ _ A) => /=[[DA' sVA]|]//=.
+    case dtB0: (tc_tree_aux _ _ B0) => /=[[DB0 sVB0]|]//=.
+    case dtB: (tc_tree_aux _ _ B) => /=[[DB sVB]|]//=.
+    case M: merge_sig => //=[S'][??]; subst.
+    have [? sA] := expand_solved_same _ eA; subst A'.
+    case eB: step => //=[B'|B'|B'|B'].
+    - have:= same_ty_tc_tree_aux sP sV A ign (maxD DB0 DB).
+      rewrite dtA.
+      case dtA1: (tc_tree_aux _ _ A) => /=[[DA1 sVA1]|]//=/eqP[?]; subst sVA1.
+      have:= same_ty_tc_tree_aux sP sVA B0 DA' DA1.
+      rewrite dtB0/=.
+      case dtB01: (tc_tree_aux _ _ B0) => /=[[DB01 sVB01]|]//=/eqP[?]; subst sVB01.
+      have:= HR _ _ _ _ _ _ dtB eB.
       admit.
-    - have [? fB]:= expand_failed_same _ e1; subst B' => +<-{r}/=.
-      rewrite fA/=sA (next_alt_not_failed fA)/=.
-      case nB0: (next_alt _ B0) => [B0'|]//=.
-        rewrite orbF/=.
-        case nA: next_alt => [A'|]//=.
-          case dtA: (tc_tree_aux _ _ A) => /=[[DA' sVA]|]//=.
-          case dtB0: (tc_tree_aux _ _ B0) => /=[[DB0 sVB0]|]//=.
-          case dtB: (tc_tree_aux _ _ B) => /=[[DB sVB]|]//=.
-          case M: merge_sig => //=[S'][??]; subst.
-          have := same_ty_tc_tree_aux sP sV A ign (maxD DB0 DB).
-          rewrite dtA; case dtA': tc_tree_aux => //=[[d2 blah]]/eqP[?]; subst blah.
-          have := same_ty_tc_tree_aux sP sVA B DA' d2.
-          rewrite dtB; case dtB': tc_tree_aux => //=[[d3 blah]]/eqP[?]; subst blah.
-          have := same_ty_tc_tree_aux sP sVA B0 DA' d2.
-          rewrite dtB0; case dtB0': tc_tree_aux => //=[[d4 blah]]/eqP[?]; subst blah.
-          rewrite M/=.
-          repeat eexists.
-          destruct DB0, DB => //=; simpl in *.
-          have /=[Sx [d'[H1 H2]]] := HL _ _ _ _ _ H dtA eA.
-          admit.
-        case nB: next_alt => [B''|]//=.
-          case dtA: (tc_tree_aux _ _ A) => /=[[DA' sVA]|]//=.
-          move=>dtB.
-          have := same_ty_tc_tree_aux sP sV A ign d.
-          rewrite dtA; case dtA': tc_tree_aux => //=[[d2 blah]]/eqP[?]; subst blah.
-          have := same_ty_tc_tree_aux sP sVA B DA' d2.
-          rewrite dtB; case dtB': tc_tree_aux => //=[[d3 blah]]/eqP[?]; subst blah.
-          repeat eexists.
-          have /=[Sx [d'[H1 H2]]] := HL _ _ _ _ _ H dtA eA.
-          destruct d => //=.
-          admit.
-        move=> [??]; subst.
-        by repeat eexists; rewrite minD_refl.
-      case nB: next_alt => [B'|]//=; last first.
-        move=> [??]; subst.
-        by repeat eexists; rewrite minD_refl.
-      rewrite orbT/= => dtB.
-      have:= same_ty_tc_tree_aux sP sV B ign d.
-      rewrite dtB; case dtB' : tc_tree_aux => /=[[DB' blah]|]//=/eqP[?]; subst blah.
-      repeat eexists.
-      destruct d => //=.
-      have [[][//_ ]] := tc_tree_aux_func2 dtB.
-      congruence.
-    - have [? sB]:= expand_solved_same _ e1; subst B'.
-      have fB:= success_failed _ sB.
-      move=> +<-{r}/=; rewrite fA sA /=.
-      rewrite (next_alt_not_failed fB) andbF/=.
-      rewrite (next_alt_not_failed fA)/=.
-      case nA: next_alt => [A'|]//=.
-        case nB0: (next_alt _ B0) => [B0'|]//=.
-          case dtA: (tc_tree_aux _ _ A) => /=[[DA' sVA]|]//=.
-          case dtB0: (tc_tree_aux _ _ B0) => /=[[DB0 sVB0]|]//=.
-          case dtB: (tc_tree_aux _ _ B) => /=[[DB sVB]|]//=.
-          case M: merge_sig => //=[S'][??]; subst.
-          have /=[Sx [d'[H1 H2]]] := HL _ _ _ _ _ H dtA eA.
-          (* have /= := HR _ _ _ _ _ _ _ dtB e1. *)
-          have:= same_ty_tc_tree_aux sP sV A ign (maxD DB0 DB).
-          rewrite dtA; case dtA' : tc_tree_aux => /=[[DA'' blah]|]//=/eqP[?]; subst blah.
-          have:= same_ty_tc_tree_aux sP sVA B0 DA' DA''.
-          rewrite dtB0; case dtB0' : tc_tree_aux => /=[[DB0'' blah]|]//=/eqP[?]; subst blah.
-          have:= same_ty_tc_tree_aux sP sVA B DA' DA''.
-          rewrite dtB; case dtB' : tc_tree_aux => /=[[DB'' blah]|]//=/eqP[?]; subst blah.
-          rewrite M/=.
-          repeat eexists.
-          destruct DB0 => //=.
-          destruct DB => //=.
-          simpl in *.
-          have [[][//_ H3]] := tc_tree_aux_func2 dtB0.
-          have [[][//_ H4]] := tc_tree_aux_func2 dtB.
-          destruct DA''.
-            have->/=: DB0'' = Func by congruence.
-            by have->/=: DB'' = Func by congruence.
-          destruct DA'; simpl in H1; subst => //=; try congruence.
-          admit. (*PB with max DB0 DB*)
-        move=> dtB.
-        have:= same_ty_tc_tree_aux sP sV B ign d.
-        rewrite dtB; case dtB' : tc_tree_aux => /=[[DB' blah]|]//=/eqP[?]; subst blah.
-        repeat eexists.
-        destruct d => //=.
-        have [[][//_ ]] := tc_tree_aux_func2 dtB.
-        congruence.
-      case nB0: (next_alt _ B0) => [B0'|]//=.
-        case dtA: (tc_tree_aux _ _ A) => /=[[DA' sVA]|]//=dtB.
-        have:= same_ty_tc_tree_aux sP sV A ign d.
-        rewrite dtA; case dtA' : tc_tree_aux => /=[[DA'' blah]|]//=/eqP[?]; subst blah.
-        have:= same_ty_tc_tree_aux sP sVA B DA' DA''.
-        rewrite dtB; case dtB' : tc_tree_aux => /=[[DB' blah]|]//=/eqP[?]; subst blah.
-        repeat eexists.
-        destruct d => //=.
-        have [[][//_ ]] := tc_tree_aux_func2 dtB.
-        destruct DA''; [congruence|].
-        destruct DA'; [|congruence].
-        have [[][//_ ]] := tc_tree_aux_func2 dtA.
-        destruct DB'; try congruence.
-      move=> H1.
-      have:= same_ty_tc_tree_aux sP sV B d ign.
-      rewrite H1; case dtB' : tc_tree_aux => /=[[DB' blah]|]//=/eqP[?]; subst blah.
-      repeat eexists.
-      destruct d => //=.
-      have [[][//]]:= tc_tree_aux_func2 H1.
-      congruence.
+    - 
+       admit.
+    - have [? fB] := expand_failed_same _ eB; subst B'.
+      have:= same_ty_tc_tree_aux sP sV A ign (maxD DB0 DB).
+      rewrite dtA.
+      case dtA1: (tc_tree_aux _ _ A) => /=[[DA1 sVA1]|]//=/eqP[?]; subst sVA1.
+      have:= same_ty_tc_tree_aux sP sVA B0 DA' DA1.
+      rewrite dtB0/=.
+      case dtB01: (tc_tree_aux _ _ B0) => /=[[DB01 sVB01]|]//=/eqP[?]; subst sVB01.
+      have:= same_ty_tc_tree_aux sP sVA B DA' DA1.
+      rewrite dtB/=.
+      case dtB1: (tc_tree_aux _ _ B) => /=[[DB1 sVB1]|]//=/eqP[?]; subst sVB1.
+      rewrite M/=; repeat eexists.
+      destruct DB0, DB => //=; simpl in *.
+      destruct DA'; simpl in *; last first.
+        have [[][// _ H1]] := tc_tree_aux_func2 dtB0.
+        move: dtB01; destruct DA1; rewrite ?dtB0?H1 => -[<-]/=; [|congruence].
+        have [[][// _ H2]] := tc_tree_aux_func2 dtB; congruence.
+      destruct ign.
+        move: dtA1; rewrite dtA => -[?]; subst.
+        move: dtB01; rewrite dtB0 => -[<-]/=; congruence.
+      have [[][//= _]] := tc_tree_aux_func2 dtA.
+      rewrite dtA1 => -[?]; subst.
+      destruct DB01;[|congruence] => /=; congruence.
+    - have [? sB]:= expand_solved_same _ eB; subst B'.
+      have:= same_ty_tc_tree_aux sP sV A ign (maxD DB0 DB).
+      rewrite dtA.
+      case dtA1: (tc_tree_aux _ _ A) => /=[[DA1 sVA1]|]//=/eqP[?]; subst sVA1.
+      have:= same_ty_tc_tree_aux sP sVA B0 DA' DA1.
+      rewrite dtB0/=.
+      case dtB01: (tc_tree_aux _ _ B0) => /=[[DB01 sVB01]|]//=/eqP[?]; subst sVB01.
+      have:= same_ty_tc_tree_aux sP sVA B DA' DA1.
+      rewrite dtB/=.
+      case dtB1: (tc_tree_aux _ _ B) => /=[[DB1 sVB1]|]//=/eqP[?]; subst sVB1.
+      rewrite M/=; repeat eexists.
+      destruct DB0, DB => //=; simpl in *.
+      destruct DA'; simpl in *; last first.
+        have [[][// _ H1]] := tc_tree_aux_func2 dtB0.
+        move: dtB01; destruct DA1; rewrite ?dtB0?H1 => -[<-]/=; [|congruence].
+        have [[][// _ H2]] := tc_tree_aux_func2 dtB; congruence.
+      destruct ign.
+        move: dtA1; rewrite dtA => -[?]; subst.
+        move: dtB01; rewrite dtB0 => -[<-]/=; congruence.
+      have [[][//= _]] := tc_tree_aux_func2 dtA.
+      rewrite dtA1 => -[?]; subst.
+      destruct DB01;[|congruence] => /=; congruence.
 Admitted.
-
-(* 
-  Given a checked program, and a deterministic tree,
-  then calling step produces a tree which is still deterministic.
-*)
-Lemma expand_det_tree1 {u sP sV sV' A r s ign d} : 
-  check_program sP ->
-    sigma2ctx sP s = Some sV ->
-      tc_tree_aux sP sV A ign = ty_ok (d, sV') ->
-        step u s A = r ->
-          exists S d', minD d d' = d' /\ sV_expand sV' S /\
-            tc_tree_aux sP sV (get_tree r) d = ty_ok (d', S).
-Proof.
-  simpl in *.
-  rewrite/check_program.
-  move=> ckP; elim: A sV sV' r s ign d.
-  - move=> sV1 sV2 r s ign d H [??] <-; subst => /=; repeat eexists; rewrite ?minD_refl//.
-    apply: sV_expand_refl.
-  - move=> sV1 sV2 r s ign d H [??] <-; subst => /=; repeat eexists; rewrite ?minD_refl//.
-    apply: sV_expand_refl.
-  - move=> sV1 sV2 r s ign d H [??] <-; subst => /=; repeat eexists; rewrite ?minD_refl//.
-    apply: sV_expand_refl.
-  - admit.
-  - move=> sV1 sV2 r s ign d H [??] <-; subst => /=; repeat eexists.
-    apply: sV_expand_refl.
-  - move=> A HA s B HB sV1 sV2 r s'/= ign d H.
-    case: (ifP (is_dead A)) => DA.
-      {
-        move=> +<-{r}; rewrite get_tree_Or/=.
-        rewrite !(is_dead_tc_tree_aux DA)//=.
-        rewrite (is_dead_next_alt _ DA)/=.
-        have? : s = s' by admit. (*should say something on the tree: I have s in the or node*)
-        subst.
-        move=> H2.
-        by have:= HB _ _ _ _ _ _ H H2 erefl.
-      }
-    case e: step => [A'|A'|A'|A']//=.
-    - have fA:= expand_not_failed _ e notF.
-      rewrite next_alt_not_failed//=.
-      move=> + <-{r}/=.
-      case nB: next_alt => [B'|]//=.
-        case dtA: (tc_tree_aux _ _ A) => /=[[DA' sVA]|]//=.
-        case dtB: (tc_tree_aux _ _ B) => /=[[DB sVB]|]//=.
-        case M: merge_sig => //=[S']; subst.
-        move=> [??]; subst.
-        case nA: next_alt => [A''|]//=; last first.
-          have:= same_ty_tc_tree_aux sP sV1 B ign (if has_cut A then maxD DA' DB else Pred).
-          rewrite dtB/=; case dtB': tc_tree_aux => //=[[D' sV']] /eqP[?]; subst.
-          repeat eexists.
-          move: dtB'.
-          case: ifP => //=cA.
-          case N: maxD => //=.
-          destruct DA', DB => //=.
-          have [[] [//= _ {}H]] := tc_tree_aux_func2 dtB.
-          rewrite H; congruence.
-          rewrite/sV_expand => k.
-          case X: lookup => //=[Se].
-          case Y: lookup => //=[Sf|].
-          admit.
-        have {HA}/=[S[d'[H1 [Hx H2]]]]:= HA _ _ _ _ _ _ H dtA e.
-        have:= same_ty_tc_tree_aux sP sV1 A' DA'(if has_cut A then maxD DA' DB else Pred).
-        rewrite H2; case dtA' : tc_tree_aux => //=[[Dx Sx]] /eqP[?]; subst Sx.
-        have:= same_ty_tc_tree_aux sP sV1 B ign (if has_cut A then maxD DA' DB else Pred).
-Abort.
 
 Definition is_det s A := forall u s' B n,
   runb u s A s' B n -> next_alt false B = None.
@@ -598,11 +246,10 @@ Proof.
     have /= [S' [d [<- H]]]:= expand_det_tree ckP H1 dtA eA; subst.
     apply: IH (H1) H.
   - move=> s1 s2 A B r n fA nA _ IH sV sV' H1 H2.
-    apply: IH (H1) _.
     have V := sigma2ctx_valid H1.
-    have := failed_det_tree_next_alt false V H2.
-    rewrite nA/= => -[d']; rewrite minD_comm/=.
-    move=> [<-{d'}]->//.
+    have := failed_det_tree_next_alt false V H2 nA.
+    move => -[[]// [s [? [X [Y Z]]]]]//.
+    apply: IH (H1) X.
   - move=> *.
     rewrite is_dead_next_alt//is_dead_dead//.
 Qed.
